WIP on accessing inductives for lob's theorem

internal/LobsTheoremProof.v
@@ -12,6 +12,7 @@ Local Open Scope positive_scope.
 Require Export Lob.quote_term.
 (*Require Export Lob.quote_has_type.*)
 Require Export Lob.conversion.
+Require Export Lob.conversion_quote.
 
 Axiom proof_admitted : False.
 Ltac admit' := case proof_admitted.
@@ -34,602 +35,383 @@ Tactic Notation "test" tactic3(tac) :=
 (** [not tac] is equivalent to [fail tac "succeeds"] if [tac] succeeds, and is equivalent to [idtac] if [tac] fails *)
 Tactic Notation "not" tactic3(tac) := try ((test tac); fail 1 tac "succeeds").
 
+Module Type Contexts.
+  Axiom qbox : Ast.term.
 
-Section quote_subst_eq.
-  Create HintDb t_quote_db discriminated.
-
-  Local Ltac t_quote0 tac :=
-    repeat match goal with
-             | _ => progress simpl
-             | _ => progress intros
-             | _ => reflexivity
-             | [ |- Ast.tApp _ _ = Ast.tApp _ _ ] => apply f_equal2; [ solve [ tac ] | ]
-             | [ |- Ast.tApp _ _ = Ast.tApp _ _ ] => apply f_equal2; [ | solve [ tac ] ]
-             | [ |- cons _ _ = cons _ _ ] => apply f_equal2
-             (*| _ => apply tApp_Proper_convertible; [ solve [ tac ] | ]
-             | _ => apply tApp_Proper_convertible; [ | solve [ tac ] ]
-             | [ |- convertible _ (Ast.tApp _ (_::_::_)%list) _ ] => apply conv_tApp_cons1
-             | [ |- convertible _ _ (Ast.tApp _ (_::_::_)%list) ] => symmetry; apply conv_tApp_cons1; symmetry*)
-             | _ => progress change conversion.convertible with convertible
-           end.
-  Local Ltac t_quote :=
-    repeat match goal with
-             | _ => progress t_quote0 t_quote
-             | _ => solve [ eauto with nocore t_quote_db ]
-           end.
-
-  Definition eq__quote_nat__closed_helper {A x}
-  : forall n n', eq (subst_n_name (quote_nat A) x n n') (quote_nat A).
-  Proof. induction A; t_quote. Qed.
-
-  Hint Resolve eq__quote_nat__closed_helper : t_quote_db.
-
-  Definition eq__quote_bool__closed_helper {A x}
-  : forall n n', eq (subst_n_name (quote_bool A) x n n') (quote_bool A).
-  Proof. induction A; t_quote. Qed.
-
-  Hint Resolve eq__quote_bool__closed_helper : t_quote_db.
-
-  Definition eq__quote_ascii__closed_helper {A x}
-  : forall n n', eq (subst_n_name (quote_ascii A) x n n') (quote_ascii A).
-  Proof. induction A; t_quote. Qed.
-
-  Hint Resolve eq__quote_ascii__closed_helper : t_quote_db.
-
-  Definition eq__quote_ident__closed_helper {A x}
-  : forall n n', eq (subst_n_name (quote_ident A) x n n') (quote_ident A).
-  Proof. induction A; t_quote. Qed.
-
-  Hint Resolve eq__quote_ident__closed_helper : t_quote_db.
-
-  Definition eq__quote_positive__closed_helper {A x}
-  : forall n n', eq (subst_n_name (quote_positive A) x n n') (quote_positive A).
-  Proof. induction A; t_quote. Qed.
-
-  Hint Resolve eq__quote_positive__closed_helper : t_quote_db.
-
-  Definition eq__quote_sort__closed_helper {A x}
-  : forall n n', eq (subst_n_name (quote_sort A) x n n') (quote_sort A).
-  Proof. induction A; t_quote. Qed.
-
-  Hint Resolve eq__quote_sort__closed_helper : t_quote_db.
-
-  Definition eq__quote_cast_kind__closed_helper {A x}
-  : forall n n', eq (subst_n_name (quote_cast_kind A) x n n') (quote_cast_kind A).
-  Proof. induction A; t_quote. Qed.
-
-  Hint Resolve eq__quote_cast_kind__closed_helper : t_quote_db.
-
-  Definition eq__quote_name__closed_helper {A x}
-  : forall n n', eq (subst_n_name (quote_name A) x n n') (quote_name A).
-  Proof. induction A; t_quote. Qed.
-
-  Hint Resolve eq__quote_name__closed_helper : t_quote_db.
-
-  Definition eq__quote_inductive__closed_helper {A x}
-  : forall n n', eq (subst_n_name (quote_inductive A) x n n') (quote_inductive A).
-  Proof. induction A; t_quote. Qed.
-
-  Hint Resolve eq__quote_inductive__closed_helper : t_quote_db.
-
-  Section sub_helpers.
-    Context (eq__quote_term__closed_helper : forall (A x : Ast.term)
-                                                    (n : option nat)
-                                                    (n' : Ast.name),
-                                               eq
-                                                 (subst_n_name
-                                                    (quote_term A) x n n')
-                                                 (quote_term A)).
-
-    Fixpoint eq__quote_term_helper__closed_helper ls x
-    : forall n n', eq (subst_n_name (quote_term_helper quote_term ls) x n n') (quote_term_helper quote_term ls).
-    Proof.
-      destruct ls as [|y ys]; simpl; try reflexivity; [].
-      intros n n'.
-      t_quote.
-    Defined.
-
-    Fixpoint eq__quote_term_helper_def__closed_helper ls x
-    : forall n n', eq (subst_n_name (quote_term_helper_def quote_term ls) x n n') (quote_term_helper_def quote_term ls).
-    Proof.
-      destruct ls as [|[] ys]; simpl; try reflexivity; [].
-      intros n n'.
-      t_quote.
-    Defined.
-  End sub_helpers.
-
-  Fixpoint eq__quote_term__closed_helper A x {struct A}
-  : forall n n', eq (subst_n_name (quote_term A) x n n') (quote_term A).
-  Proof.
-    intros n n'; destruct A; simpl;
-    repeat match goal with
-             | [ ls : list Ast.term |- _ ]
-               => unique pose proof (eq__quote_term_helper__closed_helper eq__quote_term__closed_helper ls x n n')
-             | [ ls : Ast.mfixpoint Ast.term |- _ ]
-               => unique pose proof (eq__quote_term_helper_def__closed_helper eq__quote_term__closed_helper ls x n n')
-             | [ A : Ast.term |- _ ]
-               => not constr_eq A x; unique pose proof (eq__quote_term__closed_helper A x n n')
-           end;
-    try solve [ t_quote ].
-  Defined.
-End quote_subst_eq.
-
-Section quote_has_type.
-  Local Ltac t_quote0 tac :=
-    repeat match goal with
-             | _ => progress simpl
-             | _ => progress intros
-             | _ => reflexivity
-             | [ |- has_type ?Γ (Ast.tApp ?f [?a]) ?B ]
-               => eapply (fun A => @has_type_tApp Γ f Ast.nAnon A B a)
-             | [ |- has_type ?Γ (Ast.tApp ?f [?a]) ?B ]
-               => refine (@has_type_tApp Γ f Ast.nAnon _ _ a _ _); shelve_unifiable
-             | [ |- has_type ?Γ (Ast.tApp _ (_::_::_)%list) _ ]
-               => apply has_type_tApp_split
-             | _ => exact _
-           end.
-  Local Ltac t_quote :=
-    repeat match goal with
-             | _ => progress t_quote0 t_quote
-             | _ => solve [ eauto with nocore ]
-           end.
-
-
-  Global Instance has_type__quote_nat A
-  : forall Γ, has_type Γ (quote_nat A) nat'.
-  Proof. induction A; t_quote. Qed.
-
-  Global Instance has_type__quote_bool A
-  : forall Γ, has_type Γ (quote_bool A) bool'.
-  Proof. induction A; t_quote. Qed.
-
-  Global Instance has_type__quote_ascii A
-  : forall Γ, has_type Γ (quote_ascii A) ascii'.
-  Proof. induction A; t_quote. Qed.
-
-  Global Instance has_type__quote_ident A
-  : forall Γ, has_type Γ (quote_ident A) ident'.
-  Proof. induction A; t_quote. Qed.
-
-  Global Instance has_type__quote_positive A
-  : forall Γ, has_type Γ (quote_positive A) positive'.
-  Proof. induction A; t_quote. Qed.
-
-  Global Instance has_type__quote_sort A
-  : forall Γ, has_type Γ (quote_sort A) sort'.
-  Proof. induction A; t_quote. Qed.
-
-  Global Instance has_type__quote_cast_kind A
-  : forall Γ, has_type Γ (quote_cast_kind A) cast_kind'.
-  Proof. induction A; t_quote. Qed.
-
-  Global Instance has_type__quote_name A
-  : forall Γ, has_type Γ (quote_name A) name'.
-  Proof. induction A; t_quote. Qed.
-
-  Global Instance has_type__quote_inductive A
-  : forall Γ, has_type Γ (quote_inductive A) inductive'.
-  Proof. induction A; t_quote. Qed.
-
-  Local Ltac t_has_type :=
-    repeat
-      match goal with
-        | [ |- has_type ?Γ (Ast.tApp ?f [?a]) ?B ]
-          => refine (@has_type_tApp Γ f Ast.nAnon _ _ a _ _); shelve_unifiable
-        | _ => progress simpl
-        | _ => exact _
-        | _ => apply has_type_tApp_split
-        | [ |- has_type _ (quote_term _) (subst_n_name ?e _ _ _) ]
-          => unify e term'
-        | [ |- has_type ?Γ (Ast.tApp ?f [?a]) ?B ]
-          => let A := fresh in
-             let B' := fresh in
-             evar (A : Ast.term);
-               evar (B' : Ast.term);
-               let H := fresh in
-               pose proof (@has_type_tApp Γ f Ast.nAnon A B' a) as H;
-                 subst A B';
-                 refine (_ (H _ _)); shelve_unifiable; clear H;
-                 [ | t_has_type | ]; shelve_unifiable;
-                 [ simpl; exact (fun x => x) | ]
-      end.
-
-  Section sub_helpers.
-    Context (has_type__quote_term : forall (A : Ast.term),
-                                      forall Γ, has_type Γ (quote_term A) term').
-
-    Fixpoint has_type__quote_term_helper ls
-    : forall Γ, has_type Γ (quote_term_helper quote_term ls) (Ast.tApp list' [term']).
-    Proof.
-      destruct ls as [|y ys]; simpl;
-      intro;
-      t_has_type.
-    Defined.
-
-    Fixpoint has_type__quote_term_helper_def ls
-    : forall Γ, has_type Γ (quote_term_helper_def quote_term ls) (Ast.tApp list' [Ast.tApp def' [term']]).
-    Proof.
-      destruct ls as [|[] ys]; simpl; intro; t_has_type.
-    Defined.
-  End sub_helpers.
-
-  Fixpoint has_type__quote_term A {struct A}
-  : forall Γ, has_type Γ (quote_term A) term'.
-  Proof.
-    destruct A; t_quote;
-    [ apply has_type__quote_term_helper; assumption
-    |
-    | apply has_type__quote_term_helper; assumption
-    | apply has_type__quote_term_helper_def; assumption ].
-    t_quote.
-  Qed.
-End quote_has_type.
-
-Module LC <: LobExtendedContext.
-  Definition Preterm := Ast.term.
-  Definition Context : Type := Context.
-
-  Delimit Scope context_scope with ctx.
-  Bind Scope context_scope with Context.
-
-  Definition empty_context : Context := ε.
-  Notation ε := empty_context.
-  Definition context_extend : Context -> Preterm -> Context
-    := fun Γ T => context_extend Γ (Ast.nAnon, T).
-  Notation "Γ ▻ x" := (context_extend Γ x).
-
-  Delimit Scope preterm_scope with preterm.
-  Bind Scope preterm_scope with Preterm.
-
-  Global Open Scope preterm_scope.
-
-  Definition box' (Γ : Context) (T : Preterm) : Type
-  := { t : Preterm & has_type Γ t T }.
-
-  Definition box : Preterm -> Type
-    := box' ε.
-
-  Delimit Scope well_typed_term_scope with wtt.
-  Bind Scope well_typed_term_scope with box'.
-  Bind Scope well_typed_term_scope with box.
-
-  Notation "□ T" := (box T).
-
-
-  Definition qbox : Preterm.
-  Proof.
-    let term := (eval cbv delta in box) in
-    quote_term term (fun x => exact x).
-  Defined.
-  Notation "‘□’" := qbox.
-
-  Definition tProd : Preterm -> Preterm -> Preterm
-    := Ast.tProd Ast.nAnon.
-  Notation "x ‘→’ y" := (tProd x y) : preterm_scope.
-
-  Definition tApp : Preterm -> Preterm -> Preterm
-    := fun f x => Ast.tApp f [x].
-  Notation "x ‘’ y" := (tApp x y) : preterm_scope.
-
-  Definition quote : Preterm -> Preterm
-    := quote.
-  Notation "⌜ x ⌝" := (quote x).
-
-
-  Delimit Scope well_typed_term_scope with wtt.
-  Bind Scope well_typed_term_scope with box'.
-
-  Definition is_closed (x : Preterm) : Type
-    := forall k n n', subst_n_name x k n n' = x.
+  Definition is_closed (x : Ast.term) : Type
+    := forall k n, subst_n_name x k n Ast.nAnon = x.
 
   Existing Class is_closed.
 
-  Global Instance box_is_closed : is_closed ‘□’.
-  Proof.
-    unfold qbox.
-    hnf.
-    intros k n n'.
-    destruct n; reflexivity.
-  Qed.
+  Axiom box_is_closed : is_closed qbox.
 
-  Global Instance tApp_is_closed : forall A' B', is_closed A' -> is_closed B' -> is_closed (A' ‘’ B').
-  Proof.
-    intros A' B' H0 H1 k n n'.
-    specialize (H0 k).
-    specialize (H1 k).
-    simpl; rewrite H0, H1; reflexivity.
-  Qed.
+  Axiom qquote : Ast.term.
 
-  Global Instance tProd_is_closed : forall A' B', is_closed A' -> is_closed B' -> is_closed (A' ‘→’ B').
-  Proof.
-    intros A' B' H0 H1 k n n'.
-    specialize (H0 k).
-    specialize (H1 k).
-    simpl.
-    rewrite H0, H1; reflexivity.
-  Qed.
+  Axiom qquote_is_closed : is_closed qquote.
 
-  Global Instance quote_is_closed : forall A', is_closed (quote A').
-  Proof.
-    repeat intro; apply eq__quote_term__closed_helper.
-  Qed.
-End LC.
+End Contexts.
 
-Module PRP <: PretermReflectionPrimitives LC.
-  Definition qPreterm := term'.
-  Notation "‘Preterm’" := qPreterm : preterm_scope.
+Module WithContext (Ctx : Contexts).
 
-  Global Instance has_type__quote {Γ A} : has_type Γ (quote A) qPreterm
-    := has_type__quote_term _ _.
-  Definition wttquote {Γ} A : LC.box' Γ _
-    := (quote A; has_type__quote).
-  Notation "‘⌜ A ⌝’" := (wttquote A) : well_typed_term_scope.
+  Module LC <: LobExtendedContext.
+    Definition Preterm := Ast.term.
+    Definition Context : Type := Context.
 
-  Definition qquote : LC.Preterm.
-  Proof.
-    let t := (eval cbv beta delta [qO qS qEmptyString qString qnAnon qAscii qnil qcons qmkdef qtInd qtFix qtCase qtUnknown qtRel qtConstruct qtEvar qtMeta qtVar qtApp qtConst qtSort qtCast qtProd inductive_quotable quote_ascii bool_quotable quote_bool (*quote_string quote_positive quote_nat*) ident_quotable quote_ident quote_name nat_quotable name_quotable quote quote_term sort_quotable cast_kind_quotable quote_sort qsSet qsProp qsType universe_quotable quote_inductive qmkInd] in quote_term) in
-    quote_term t (fun x => exact x).
-  Defined.
-  Notation "‘quote’" := qquote : preterm_scope.
-End PRP.
+    Delimit Scope context_scope with ctx.
+    Bind Scope context_scope with Context.
 
-Module PP <: PretermPrimitives LC.
-  Export LC PRP.
-  Definition tLambda : Preterm -> Preterm -> Preterm
-    := Ast.tLambda Ast.nAnon.
-  Definition qtApp : Preterm
-    := tLambda ‘Preterm’ (tLambda ‘Preterm’ (Ast.tApp qtApp [Ast.tRel 1; (Ast.tApp qcons [‘Preterm’; Ast.tRel 0; Ast.tApp qnil [‘Preterm’]])])).
+    Definition empty_context : Context := DefaultContext.
+    Notation ε := empty_context.
 
-  Notation "‘App’" := qtApp : preterm_scope.
+    Definition context_extend : Context -> Preterm -> Context
+      := fun Γ T => context_extend Γ (CBinder Ast.nAnon T).
+    Notation "Γ ▻ x" := (context_extend Γ x).
 
-  Definition qtProd : Preterm -> Preterm -> Preterm
-    := fun A B => (qtProd ‘’ qnAnon ‘’ A ‘’ B)%preterm.
-  Notation "x ‘‘→’’ y" := (qtProd x y) : preterm_scope.
+    Delimit Scope preterm_scope with preterm.
+    Bind Scope preterm_scope with Preterm.
 
-  Definition tVar0 : Preterm
-    := Ast.tRel 0.
-  Notation "‘VAR₀’" := tVar0.
+    Global Open Scope preterm_scope.
 
-  Definition ttVar0 {Γ T} : box' (Γ ▻ T) T.
-  Proof.
-    refine (tVar0; _).
-    apply has_type_tRel_0.
-  Defined.
-  Notation "‘‘VAR₀’’" := ttVar0 : well_typed_term_scope.
-End PP.
+    Definition box' (Γ : Context) (T : Preterm) : Type
+      := { t : Preterm & has_type Γ t T }.
 
-Module TR <: TypingRules LC PP.
-  Export LC PP.
-  Definition capture_avoiding_subst_0 : forall (in_term : Preterm)
-                                               (new_value : Preterm),
-                                          Preterm
-    := fun in_term new_value
-       => subst_n_name in_term new_value (Some 0%nat) Ast.nAnon.
-  Notation "x [ 0 ↦ y ]" := (capture_avoiding_subst_0 x y).
-  Global Arguments capture_avoiding_subst_0 !_ / _.
-  Definition convertible : Context -> Preterm -> Preterm -> Type
-    := convertible.
+    Definition box : Preterm -> Type
+      := box' ε.
 
-  Definition eq__subst__quote
-  : forall A x, capture_avoiding_subst_0 (quote A) x = quote A.
-  Proof.
-    intros; unfold quote, capture_avoiding_subst_0.
-    rewrite eq__quote_term__closed_helper; reflexivity.
-  Defined.
+    Delimit Scope well_typed_term_scope with wtt.
+    Bind Scope well_typed_term_scope with box'.
+    Bind Scope well_typed_term_scope with box.
 
-  Definition box'_respectful : forall {Γ A B},
-                                 convertible Γ A B
-                                 -> box' Γ A
-                                 -> box' Γ B.
-  Proof.
-    intros Γ A B H [a Ha].
-    exists a.
-    eapply has_type_conv_subst; try eassumption.
-  Defined.
+    Notation "□ T" := (box T).
 
-  Global Instance convertible_refl : forall {Γ}, Reflexive (convertible Γ) := conv_refl.
-  Global Instance convertible_sym : forall {Γ}, Symmetric (convertible Γ) := conv_sym.
-  Global Instance convertible_trans : forall {Γ}, Transitive (convertible Γ) := conv_trans.
-  Definition convertible_beta_app_lambda
-  : forall Γ A f a,
-      convertible Γ (tApp (tLambda A f) a) (capture_avoiding_subst_0 f a).
-  Proof.
-    intros; eapply conv_beta.
-  Defined.
-  Definition convertible__capture_avoiding_subst_0__tApp
-  : forall Γ A B x,
-      convertible Γ ((A ‘’ B) [ 0 ↦ x ]) ((A [ 0 ↦ x ]) ‘’ (B [ 0 ↦ x ])).
-  Proof.
-    reflexivity.
-  Defined.
-  Definition convertible__capture_avoiding_subst_0__qtProd
-  : forall Γ A B x,
-      convertible Γ ((A ‘‘→’’ B) [ 0 ↦ x ]) ((A [ 0 ↦ x ]) ‘‘→’’ (B [ 0 ↦ x ])).
-  Proof.
-    reflexivity.
-  Defined.
-  Definition convertible__capture_avoiding_subst_0__tVar0
-  : forall Γ x,
-      convertible Γ (‘VAR₀’ [ 0 ↦ x ]) x.
-  Proof.
-    reflexivity.
-  Defined.
 
-  Global Instance tApp_Proper_convertible
-  : forall Γ,
-      Proper (convertible Γ ==> convertible Γ ==> convertible Γ) tApp.
-  Proof.
-    repeat intro; apply conv_tApp_respectful; assumption.
-  Defined.
-  Global Instance qtProd_Proper_convertible
-  : forall Γ,
-      Proper (convertible Γ ==> convertible Γ ==> convertible Γ) qtProd.
-  Proof.
-    repeat intro.
-    unfold qtProd.
-    apply tApp_Proper_convertible; [ | assumption ].
-    apply tApp_Proper_convertible; [ reflexivity | assumption ].
-  Defined.
-  Global Instance tProd_Proper_convertible
-  : forall Γ,
-      Proper (convertible Γ ==> eq ==> convertible Γ) tProd.
-  Proof.
-    repeat intro.
-    apply conv_tProd_respectful; [ assumption | subst; reflexivity ].
-  Defined.
-  Definition convertible__quote__qtProd
-  : forall Γ A B,
-      convertible Γ (⌜ A ‘→’ B ⌝) (⌜ A ⌝ ‘‘→’’ ⌜ B ⌝).
-  Proof.
-    repeat intro.
-    simpl.
-    unfold qtProd, tApp; simpl.
-    symmetry.
-    apply conv_tApp_cons2.
-    apply conv_tApp_cons2.
-    reflexivity.
-  Defined.
+    Definition qbox : Preterm := Ctx.qbox.
+    Notation "‘□’" := qbox.
 
-  Definition convertible__qtApp__closed
-  : forall Γ x,
-      convertible Γ (‘App’ [ 0 ↦ x ]) (‘App’).
-  Proof.
-    reflexivity.
-  Defined.
+    Definition tProd : Preterm -> Preterm -> Preterm
+      := Ast.tProd Ast.nAnon.
+    Notation "x ‘→’ y" := (tProd x y) : preterm_scope.
 
-  Definition convertible__quote__closed
-  : forall Γ A x,
-      convertible Γ ((quote A) [ 0 ↦ x ]) (quote A).
-  Proof.
-    intros; rewrite eq__subst__quote.
-    reflexivity.
-  Defined.
+    Definition tApp : Preterm -> Preterm -> Preterm
+      := fun f x => Ast.tApp f [x].
+    Notation "x ‘’ y" := (tApp x y) : preterm_scope.
 
-  Hint Resolve convertible__quote__closed : t_quote_db.
+    Definition quote : Preterm -> Preterm
+      := quote.
+    Notation "⌜ x ⌝" := (quote x).
 
-  Definition convertible__quote__app
-  : forall Γ A B,
-      convertible Γ (⌜ A ‘’ B ⌝) ((‘App’ ‘’ ⌜ A ⌝) ‘’ ⌜ B ⌝).
-  Proof.
-    intros; simpl.
-    unfold tApp, qtApp, tLambda.
-    symmetry.
-    etransitivity.
-    { apply conv_tApp_respectful; [ | reflexivity ].
-      apply conv_beta. }
-    simpl.
-    etransitivity; [ apply conv_beta | ].
-    simpl.
-    unfold capture_avoiding_subst_0.
-    rewrite eq__quote_term__closed_helper; reflexivity.
-  Defined.
 
-End TR.
+    Delimit Scope well_typed_term_scope with wtt.
+    Bind Scope well_typed_term_scope with box'.
 
-Module PreL' <: PreL LC PP.
-  Export LC PP.
+    Definition is_closed (x : Preterm) : Type
+      := forall k n, subst_n_name x k n Ast.nAnon = x.
 
-  Definition wttLambda_nd
-             {Γ : Context} {B' : Preterm}
-  : forall A' : Preterm, box' (Γ ▻ A') B' -> box' Γ (A' ‘→’ B').
-  Proof.
-    refine (fun A' body
-            => (Ast.tLambda Ast.nAnon A' body.1;
-                _)).
-    apply has_type_tLambda.
-    exact body.2.
-  Defined.
+    Existing Class is_closed.
 
-  Definition wttApp_1 {Γ : Context} {A' B' : Preterm}
-  : box' Γ (A' ‘→’ B')
-    -> forall x : box' Γ A',
-         box' Γ (subst_n_name B' x.1 (Some 0%nat) Ast.nAnon).
-  Proof.
-    refine (fun F x
-            => (Ast.tApp F.1 [x.1];
-                _)).
-    eapply has_type_tApp.
-    { exact F.2. }
-    { exact x.2. }
-  Defined.
+    Global Instance box_is_closed : is_closed ‘□’
+      := Ctx.box_is_closed.
 
-  Definition wttApp_1_nd {Γ : Context} {A' B' : Preterm} {H : is_closed B'}
-  : box' Γ (A' ‘→’ B') -> box' Γ A' -> box' Γ B'.
-  Proof.
-    intros F x.
-    pose proof (wttApp_1 F x) as H'.
-    exists H'.1.
-    destruct H' as [Fx H']; simpl.
-    hnf in H.
-    rewrite H in H'.
-    apply H'.
-  Defined.
+    Global Instance tApp_is_closed : forall A' B', is_closed A' -> is_closed B' -> is_closed (A' ‘’ B').
+    Proof.
+      intros A' B' H0 H1 k n.
+      specialize (H0 k).
+      specialize (H1 k).
+      simpl; rewrite H0, H1; reflexivity.
+    Qed.
 
-  Notation "x ‘’ y" := (wttApp_1_nd x%wtt y%wtt) : well_typed_term_scope.
-End PreL'.
+    Global Instance tProd_is_closed : forall A' B', is_closed A' -> is_closed B' -> is_closed (A' ‘→’ B').
+    Proof.
+      intros A' B' H0 H1 k n.
+      specialize (H0 k).
+      specialize (H1 k).
+      simpl.
+      rewrite H0, H1; reflexivity.
+    Qed.
 
-Module Type DoublyQuotedThings.
-  Export TR LC PP PRP.
-  Axiom qbox_Ui : Ast.sort.
-  Axiom has_type_qbox
-  : has_type ε ‘□’ (term' ‘→’ Ast.tSort qbox_Ui).
-  Global Existing Instance has_type_qbox.
+    Global Instance quote_is_closed : forall A', is_closed (quote A').
+    Proof.
+      repeat intro; apply eq__quote_term__closed_helper.
+    Qed.
+  End LC.
 
-  Axiom box_qtProd_dom_precompose
-  : forall {Γ} A B C,
-      (box' Γ (‘□’ ‘’ B) -> box' Γ (‘□’ ‘’ A))
-      -> box' Γ (‘□’ ‘’ (A ‘‘→’’ C))
-      -> box' Γ (‘□’ ‘’ (B ‘‘→’’ C)).
+  Module PRP <: PretermReflectionPrimitives LC.
+    Definition qPreterm := term'.
+    Notation "‘Preterm’" := qPreterm : preterm_scope.
 
-  (** FIXME: This seems a bit fishy... *)
-  Axiom box_quote_app_quote
-  : forall Γ T,
-      box' Γ (‘□’
-               ‘’ (‘App’ ‘’ ⌜‘□’ ⌝ ‘’ (‘App’ ‘’ ⌜T ⌝ ‘’ (‘App’ ‘’ ⌜ ‘quote’ ⌝ ‘’ ⌜ T ⌝))))
-      -> box' Γ (‘□’ ‘’ (‘App’ ‘’ ⌜‘□’ ⌝ ‘’ (‘App’ ‘’ ⌜T ⌝ ‘’ ⌜ ⌜ T ⌝ ⌝))).
+    Global Instance has_type__quote {Γ A} : has_type _ (quote A) qPreterm
+      := has_type__quote_term _ Γ.
+    Definition wttquote {Γ} A : LC.box' _ _
+      := (quote A; @has_type__quote Γ _).
+    Notation "‘⌜ A ⌝’" := (wttquote A) : well_typed_term_scope.
 
-  Axiom box_quote_app_quote_inv
-  : forall Γ T,
-      box' Γ (‘□’ ‘’ (‘App’ ‘’ ⌜‘□’ ⌝ ‘’ (‘App’ ‘’ ⌜T ⌝ ‘’ ⌜ ⌜ T ⌝ ⌝)))
-      -> box' Γ (‘□’
-                  ‘’ (‘App’ ‘’ ⌜‘□’ ⌝ ‘’ (‘App’ ‘’ ⌜T ⌝ ‘’ (‘App’ ‘’ ⌜ ‘quote’ ⌝ ‘’ ⌜ T ⌝)))).
+    Definition qquote : LC.Preterm
+      := Ctx.qquote.
+    (*Proof.
+      let t := (eval cbv beta delta [qO qS qEmptyString qString qnAnon qAscii qnil qcons qmkdef qtInd qtFix qtCase qtUnknown qtRel qtConstruct qtEvar qtMeta qtVar qtApp qtConst qtSort qtCast qtProd inductive_quotable quote_ascii bool_quotable quote_bool (*quote_string quote_positive quote_nat*) ident_quotable quote_ident quote_name nat_quotable name_quotable quote quote_term sort_quotable cast_kind_quotable quote_sort qsSet qsProp qsType universe_quotable quote_inductive qmkInd] in quote_term) in
+      quote_term t (fun x => exact x).
+    Defined.*)
+    Notation "‘quote’" := qquote : preterm_scope.
+  End PRP.
 
-  Axiom Quot : forall T, □ T -> □ (‘□’ ‘’ ⌜ T ⌝).
+  Module PP <: PretermPrimitives LC.
+    Export LC PRP.
+    Definition tLambda : Preterm -> Preterm -> Preterm
+      := Ast.tLambda Ast.nAnon.
+    Definition qtApp : Preterm
+      := tLambda ‘Preterm’ (tLambda ‘Preterm’ (Ast.tApp qtApp [Ast.tRel 1; (Ast.tApp qcons [‘Preterm’; Ast.tRel 0; Ast.tApp qnil [‘Preterm’]])])).
 
-  Section context.
-    Context (qX qL0 : Preterm).
-    Let Γ := (ε ▻ (‘□’
-                    ‘’ (tLambda ‘Preterm’
-                                (‘App’ ‘’ ⌜ ‘□’ ⌝
-                                  ‘’ (‘App’ ‘’ ‘VAR₀’ ‘’ (‘App’ ‘’ ⌜ ‘quote’ ⌝ ‘’ ‘VAR₀’))
-                                  ‘‘→’’ ⌜ qX ⌝) ‘’ ⌜ qL0 ⌝))).
+    Notation "‘App’" := qtApp : preterm_scope.
 
-    Axiom qQuote
-    : forall T,
-        let A := (‘□’ ‘’ T)%preterm in
-        box' Γ (A ‘→’ (‘□’ ‘’ (⌜ A ⌝))).
+    Definition qtProd : Preterm -> Preterm -> Preterm
+      := fun A B => (qtProd ‘’ qnAnon ‘’ A ‘’ B)%preterm.
+    Notation "x ‘‘→’’ y" := (qtProd x y) : preterm_scope.
 
-    Axiom qbApp
-    : forall A' B',
-        box' Γ ((‘□’ ‘’ (A' ‘‘→’’ B')) ‘→’ (‘□’ ‘’ A') ‘→’ (‘□’ ‘’ B')).
-  End context.
-End DoublyQuotedThings.
+    Definition tVar0 : Preterm
+      := Ast.tRel 0.
+    Notation "‘VAR₀’" := tVar0.
 
-Module PRTR (DQT : DoublyQuotedThings) <: PretermReflectionTypingRules LC PP PRP TR.
-  Export LC PP PRP TR.
-  Include DQT.
-  Definition convertible__qquote__closed
-  : forall Γ x,
-      convertible Γ (‘quote’ [ 0 ↦ x ]) (‘quote’).
-  Proof.
-    reflexivity.
-  Defined.
-End PRTR.
+    Definition ttVar0 {Γ T} : box' (Γ ▻ T) T.
+    Proof.
+      refine (tVar0; _).
+      apply has_type_tRel_0.
+    Defined.
+    Notation "‘‘VAR₀’’" := ttVar0 : well_typed_term_scope.
+  End PP.
 
-Local Ltac t_has_type :=
-  repeat
-    repeat
+  Module TR <: TypingRules LC PP.
+    Export LC PP.
+    Definition capture_avoiding_subst_0 : forall (in_term : Preterm)
+                                                 (new_value : Preterm),
+                                            Preterm
+      := fun in_term new_value
+         => subst_n_name in_term new_value (Some 0%nat) Ast.nAnon.
+    Notation "x [ 0 ↦ y ]" := (capture_avoiding_subst_0 x y).
+    Global Arguments capture_avoiding_subst_0 !_ / _.
+    Definition convertible : Context -> Preterm -> Preterm -> Type
+      := convertible.
+
+    Definition eq__subst__quote
+    : forall A x, capture_avoiding_subst_0 (quote A) x = quote A.
+    Proof.
+      intros; unfold quote, capture_avoiding_subst_0.
+      rewrite eq__quote_term__closed_helper; reflexivity.
+    Defined.
+
+    Definition box'_respectful : forall {Γ A B},
+                                   convertible Γ A B
+                                   -> box' Γ A
+                                   -> box' Γ B.
+    Proof.
+      intros Γ A B H [a Ha].
+      exists a.
+      eapply has_type_conv_subst; try eassumption.
+    Defined.
+
+    Global Instance convertible_refl : forall {Γ}, Reflexive (convertible Γ) := conv_refl.
+    Global Instance convertible_sym : forall {Γ}, Symmetric (convertible Γ) := conv_sym.
+    Global Instance convertible_trans : forall {Γ}, Transitive (convertible Γ) := conv_trans.
+    Definition convertible_beta_app_lambda
+    : forall Γ A f a,
+        convertible Γ (tApp (tLambda A f) a) (capture_avoiding_subst_0 f a).
+    Proof.
+      intros; eapply conv_beta.
+    Defined.
+    Definition convertible__capture_avoiding_subst_0__tApp
+    : forall Γ A B x,
+        convertible Γ ((A ‘’ B) [ 0 ↦ x ]) ((A [ 0 ↦ x ]) ‘’ (B [ 0 ↦ x ])).
+    Proof.
+      reflexivity.
+    Defined.
+    Definition convertible__capture_avoiding_subst_0__qtProd
+    : forall Γ A B x,
+        convertible Γ ((A ‘‘→’’ B) [ 0 ↦ x ]) ((A [ 0 ↦ x ]) ‘‘→’’ (B [ 0 ↦ x ])).
+    Proof.
+      reflexivity.
+    Defined.
+    Definition convertible__capture_avoiding_subst_0__tVar0
+    : forall Γ x,
+        convertible Γ (‘VAR₀’ [ 0 ↦ x ]) x.
+    Proof.
+      reflexivity.
+    Defined.
+
+    Global Instance tApp_Proper_convertible
+    : forall Γ,
+        Proper (convertible Γ ==> convertible Γ ==> convertible Γ) tApp.
+    Proof.
+      repeat intro; apply conv_tApp_respectful; assumption.
+    Defined.
+    Global Instance qtProd_Proper_convertible
+    : forall Γ,
+        Proper (convertible Γ ==> convertible Γ ==> convertible Γ) qtProd.
+    Proof.
+      repeat intro.
+      unfold qtProd.
+      apply tApp_Proper_convertible; [ | assumption ].
+      apply tApp_Proper_convertible; [ reflexivity | assumption ].
+    Defined.
+    Global Instance tProd_Proper_convertible
+    : forall Γ,
+        Proper (convertible Γ ==> eq ==> convertible Γ) tProd.
+    Proof.
+      repeat intro.
+      apply conv_tProd_respectful; [ assumption | subst; reflexivity ].
+    Defined.
+    Definition convertible__quote__qtProd
+    : forall Γ A B,
+        convertible Γ (⌜ A ‘→’ B ⌝) (⌜ A ⌝ ‘‘→’’ ⌜ B ⌝).
+    Proof.
+      repeat intro.
+      simpl.
+      unfold qtProd, tApp; simpl.
+      symmetry.
+      apply conv_tApp_cons2.
+      apply conv_tApp_cons2.
+      reflexivity.
+    Defined.
+
+    Definition convertible__qtApp__closed
+    : forall Γ x,
+        convertible Γ (‘App’ [ 0 ↦ x ]) (‘App’).
+    Proof.
+      reflexivity.
+    Defined.
+
+    Definition convertible__quote__closed
+    : forall Γ A x,
+        convertible Γ ((quote A) [ 0 ↦ x ]) (quote A).
+    Proof.
+      intros; rewrite eq__subst__quote.
+      reflexivity.
+    Defined.
+
+    Hint Resolve convertible__quote__closed : t_quote_db.
+
+    Definition convertible__quote__app
+    : forall Γ A B,
+        convertible Γ (⌜ A ‘’ B ⌝) ((‘App’ ‘’ ⌜ A ⌝) ‘’ ⌜ B ⌝).
+    Proof.
+      intros; simpl.
+      unfold tApp, qtApp, tLambda.
+      symmetry.
+      etransitivity.
+      { apply conv_tApp_respectful; [ | reflexivity ].
+        apply conv_beta. }
+      simpl.
+      etransitivity; [ apply conv_beta | ].
+      simpl.
+      unfold capture_avoiding_subst_0.
+      rewrite eq__quote_term__closed_helper; reflexivity.
+    Defined.
+
+  End TR.
+
+  Module PreL' <: PreL LC PP.
+    Export LC PP.
+
+    Definition wttLambda_nd
+               {Γ : Context} {B' : Preterm}
+    : forall A' : Preterm, box' (Γ ▻ A') B' -> box' Γ (A' ‘→’ B').
+    Proof.
+      refine (fun A' body
+              => (Ast.tLambda Ast.nAnon A' body.1;
+                  _)).
+      apply has_type_tLambda.
+      exact body.2.
+    Defined.
+
+    Definition wttApp_1 {Γ : Context} {A' B' : Preterm}
+    : box' Γ (A' ‘→’ B')
+      -> forall x : box' Γ A',
+           box' Γ (subst_n_name B' x.1 (Some 0%nat) Ast.nAnon).
+    Proof.
+      refine (fun F x
+              => (Ast.tApp F.1 [x.1];
+                  _)).
+      eapply has_type_tApp.
+      { exact F.2. }
+      { exact x.2. }
+    Defined.
+
+    Definition wttApp_1_nd {Γ : Context} {A' B' : Preterm} {H : is_closed B'}
+    : box' Γ (A' ‘→’ B') -> box' Γ A' -> box' Γ B'.
+    Proof.
+      intros F x.
+      pose proof (wttApp_1 F x) as H'.
+      exists H'.1.
+      destruct H' as [Fx H']; simpl.
+      hnf in H.
+      rewrite H in H'.
+      apply H'.
+    Defined.
+
+    Notation "x ‘’ y" := (wttApp_1_nd x%wtt y%wtt) : well_typed_term_scope.
+  End PreL'.
+
+  Module Type DoublyQuotedThings.
+    Export TR LC PP PRP.
+    Axiom qbox_Ui : Ast.sort.
+    Axiom has_type_qbox
+    : has_type ε ‘□’ (term' ‘→’ Ast.tSort qbox_Ui).
+    Global Existing Instance has_type_qbox.
+
+    Axiom box_qtProd_dom_precompose
+    : forall {Γ} A B C,
+        (box' Γ (‘□’ ‘’ B) -> box' Γ (‘□’ ‘’ A))
+        -> box' Γ (‘□’ ‘’ (A ‘‘→’’ C))
+        -> box' Γ (‘□’ ‘’ (B ‘‘→’’ C)).
+
+    (** FIXME: This seems a bit fishy... *)
+    Axiom box_quote_app_quote
+    : forall Γ T,
+        box' Γ (‘□’
+                 ‘’ (‘App’ ‘’ ⌜‘□’ ⌝ ‘’ (‘App’ ‘’ ⌜T ⌝ ‘’ (‘App’ ‘’ ⌜ ‘quote’ ⌝ ‘’ ⌜ T ⌝))))
+        -> box' Γ (‘□’ ‘’ (‘App’ ‘’ ⌜‘□’ ⌝ ‘’ (‘App’ ‘’ ⌜T ⌝ ‘’ ⌜ ⌜ T ⌝ ⌝))).
+
+    Axiom box_quote_app_quote_inv
+    : forall Γ T,
+        box' Γ (‘□’ ‘’ (‘App’ ‘’ ⌜‘□’ ⌝ ‘’ (‘App’ ‘’ ⌜T ⌝ ‘’ ⌜ ⌜ T ⌝ ⌝)))
+        -> box' Γ (‘□’
+                    ‘’ (‘App’ ‘’ ⌜‘□’ ⌝ ‘’ (‘App’ ‘’ ⌜T ⌝ ‘’ (‘App’ ‘’ ⌜ ‘quote’ ⌝ ‘’ ⌜ T ⌝)))).
+
+    Axiom Quot : forall T, □ T -> □ (‘□’ ‘’ ⌜ T ⌝).
+
+    Section context.
+      Context (qX qL0 : Preterm).
+      Let Γ := (ε ▻ (‘□’
+                      ‘’ (tLambda ‘Preterm’
+                                  (‘App’ ‘’ ⌜ ‘□’ ⌝
+                                    ‘’ (‘App’ ‘’ ‘VAR₀’ ‘’ (‘App’ ‘’ ⌜ ‘quote’ ⌝ ‘’ ‘VAR₀’))
+                                    ‘‘→’’ ⌜ qX ⌝) ‘’ ⌜ qL0 ⌝))).
+
+      Axiom qQuote
+      : forall T,
+          let A := (‘□’ ‘’ T)%preterm in
+          box' Γ (A ‘→’ (‘□’ ‘’ (⌜ A ⌝))).
+
+      Axiom qbApp
+      : forall A' B',
+          box' Γ ((‘□’ ‘’ (A' ‘‘→’’ B')) ‘→’ (‘□’ ‘’ A') ‘→’ (‘□’ ‘’ B')).
+    End context.
+  End DoublyQuotedThings.
+
+  Module PRTR (DQT : DoublyQuotedThings) <: PretermReflectionTypingRules LC PP PRP TR.
+    Export LC PP PRP TR.
+    Include DQT.
+    Definition convertible__qquote__closed
+    : forall Γ x,
+        convertible Γ (‘quote’ [ 0 ↦ x ]) (‘quote’).
+    Proof.
+      unfold capture_avoiding_subst_0; intros.
+      rewrite Ctx.qquote_is_closed; reflexivity.
+    Defined.
+  End PRTR.
+
+  Local Ltac t_has_type' :=
+    idtac;
     match goal with
+      | _ => progress simpl in *
       | _ => exact _
       | [ |- has_type _ (Ast.tLambda (Ast.nNamed _) _ _) _ ]
         => apply has_type_tLambda_unname
@@ -641,6 +423,12 @@ Local Ltac t_has_type :=
         => refine (has_type_tProd _ _ _ _ _ _); shelve_unifiable
       | [ |- has_type _ (quote_term _) (subst_n_name ?e _ _ _) ]
         => unify e term'
+      | [ |- has_type _ (Ast.tApp (Ast.tLambda _ _ _) [_]) _ ]
+        => eapply has_type_conv_subst_term;
+          [
+          | symmetry; solve [ apply conv_beta ] ];
+          simpl subst_n_name
+      | _ => rewrite !eq__quote_term__closed_helper
       | [ |- has_type ?Γ (Ast.tApp ?f [?a]) ?B ]
         => let A := fresh in
            let B' := fresh in
@@ -650,11 +438,28 @@ Local Ltac t_has_type :=
              pose proof (@has_type_tApp Γ f Ast.nAnon A B' a) as H;
                subst A B';
                refine (_ (H _ _)); shelve_unifiable; clear H;
-               [ | t_has_type | ]; shelve_unifiable;
+               [ | repeat t_has_type' | ]; shelve_unifiable;
                [ simpl; exact (fun x => x) | ]
       | _ => exact _
       | [ |- has_type ?Γ (Ast.tApp ?f [?a]) ?B ]
         => not is_evar B; eapply has_type_conv_subst; shelve_unifiable
+      | [ |- has_type (_ ▻▻ _) _ _ ]
+        => apply wkg_rel_free; [ intros ? [?|]; reflexivity | intros ? [?|]; reflexivity | ]
+      | [ |- has_type _ _ _ ]
+        => eapply has_type_conv_subst;
+          [ eapply has_type_tConstruct1_Lookup;
+            [ | | simpl; reflexivity ];
+            hnf; simpl; reflexivity
+          | ]
+      | [ |- convertible ?Γ ?k _ ] => unfold k
+      | [ |- convertible ?Γ (Ast.tConst ?n) _ ]
+        => let H := fresh in
+           pose proof (@conv_delta_Lookup Γ n) as H;
+             unfold is_rel_free in H;
+             simpl in H;
+             apply (H (fun _ _ => eq_refl))
+      | [ |- conversion.convertible _ (Ast.tProd _ _ _) (Ast.tProd _ _ _) ]
+        => apply conv_tProd_respectful
       | _ => progress simpl
       | [ |- has_type _ (Ast.tApp _ (_::_::_)%list) _ ]
         => apply has_type_tApp_split
@@ -679,234 +484,325 @@ Local Ltac t_has_type :=
 
 
 
-Module LA (DQT : DoublyQuotedThings) <: PostL_Assumptions LC PP PRP TR.
-  Export TR LC PP PRP.
-  Include DQT.
+  Module LA (DQT : DoublyQuotedThings) <: PostL_Assumptions LC PP PRP TR.
+    Export TR LC PP PRP.
+    Include DQT.
 
-  Section context.
-    Context (qX qL0 : Preterm).
-    Let Γ := (ε ▻ (‘□’
-                    ‘’ (tLambda ‘Preterm’
-                                (‘App’ ‘’ ⌜ ‘□’ ⌝
-                                  ‘’ (‘App’ ‘’ ‘VAR₀’ ‘’ (‘App’ ‘’ ⌜ ‘quote’ ⌝ ‘’ ‘VAR₀’))
-                                  ‘‘→’’ ⌜ qX ⌝) ‘’ ⌜ qL0 ⌝))).
+    Section context.
+      Context (qX qL0 : Preterm).
+      Let Γ := (ε ▻ (‘□’
+                      ‘’ (tLambda ‘Preterm’
+                                  (‘App’ ‘’ ⌜ ‘□’ ⌝
+                                    ‘’ (‘App’ ‘’ ‘VAR₀’ ‘’ (‘App’ ‘’ ⌜ ‘quote’ ⌝ ‘’ ‘VAR₀’))
+                                    ‘‘→’’ ⌜ qX ⌝) ‘’ ⌜ qL0 ⌝))).
 
-    Definition box'_weaken
-    : forall {A}, box' ε A -> box' Γ A.
+      Definition box'_weaken
+      : forall {A} {H : is_closed A}, box' ε A -> box' Γ A.
+      Proof.
+        simpl; intros A H bA.
+        refine (bump_rel_from bA.1 (Some 0%nat) Ast.nAnon tt; _).
+        apply is_rel_free_iff in H.
+        hnf in H.
+        rewrite <- (H (Some 0%nat)).
+        subst Γ.
+        eapply (wkg_1 (Δ := nil)); [ | exact bA.2 ].
+        unfold qtProd, qtApp, tApp, tLambda.
+        Time do 3 t_has_type'.
+        { match goal with
+      | [ |- has_type ?Γ (Ast.tApp ?f [?a]) ?B ]
+        => let A := fresh in
+           let B' := fresh in
+           evar (A : Ast.term);
+             evar (B' : Ast.term);
+             let H := fresh in
+             pose proof (@has_type_tApp Γ f Ast.nAnon A B' a) as H;
+               subst A B';
+               refine (_ (H _ _)); shelve_unifiable; clear H;
+               [ |  | ]; shelve_unifiable;
+               [ simpl | | ]
+end.
+Focus 2.
+{
+        { match goal with
+      | [ |- has_type ?Γ (Ast.tApp ?f [?a]) ?B ]
+        => let A := fresh in
+           let B' := fresh in
+           evar (A : Ast.term);
+             evar (B' : Ast.term);
+             let H := fresh in
+             pose proof (@has_type_tApp Γ f Ast.nAnon A B' a) as H;
+               subst A B';
+               refine (_ (H _ _)); shelve_unifiable; clear H;
+               [ |  | ]; shelve_unifiable;
+               [ simpl | | ]
+end.
+Focus 2.
+{ repeat t_has_type'. }
+Unfocus.
+{ Time do 5 t_has_type'. }
+{ Time do 2 t_has_type'.
+{ t_has_type'.
+t_has_type'.
+t_has_type'.
+t_has_type'.
+t_has_type'.
+t_has_type'.
+t_has_type'.
+t_has_type'.
+t_has_type'.
+t_has_type'.
+t_has_type'.
+t_has_type'.
+t_has_type'.
+t_has_type'.
+t_has_type'.
+
+Existing Class eq.
+Hint Extern 1 (Some (CType ?x _) = Some (CType ?x _)) => reflexivity : typeclass_instances.
+
+eapply has_type_tConstruct1_Lookup; simpl.
+
+3:exact _.
+simpl.
+all:simpl; try exact _.
+all:simpl; try exact _.
+t_has_type'.
+t_has_type'.
+Global Existing Instance has_type__quote_term_1
+refine (@has_type__quote_term _ [(_, _)]%list).
+
+rewrite eq__quote_term__closed_helper.
+
+        {
+
+
+
+          all:admit. }
+        {
+
+admit'.
+        (* refine ((fun Ui H => @wkg_1_nil nil Ast.nAnon _ _ _ Ui H bA.2) _ _); shelve_unifiable.
+        unfold qtProd, qtApp, tApp, tLambda.
+        t_has_type.*)
+      Qed.
+    End context.
+
+    Definition App : forall {A' B'} {H : is_closed B'},
+                       □ (A' ‘→’ B') -> □ A' -> □ B'.
     Proof.
-      simpl; intros A bA.
-      refine (bA.1; _).
-      refine ((fun Ui H => @wkg_1_nil nil Ast.nAnon _ _ _ Ui H bA.2) _ _); shelve_unifiable.
-      unfold qtProd, qtApp, tApp, tLambda.
-      t_has_type.
+      intros A' B' H AtoB A.
+      refine (AtoB.1 ‘’ A.1;
+              _ (has_type_tApp ε AtoB.1 Ast.nAnon A' B' A.1 AtoB.2 A.2)).
+      clear -H; abstract (hnf in H; rewrite H; intro; assumption).
+    Defined.
+  End LA.
+
+  Module Lob (LH : LobHypotheses LC) (DQT : DoublyQuotedThings) <: LobsTheorem LC LH.
+    Module PRTR' := PRTR DQT.
+    Module LA' := LA DQT.
+    Module Lob' := LobOfPreLob LC LH PP PreL' PRP TR PRTR' LA'.
+    Definition lob := Lob'.lob.
+    Print Assumptions lob.
+  End Lob.
+End WithContext.
+
+
+  Module DQT <: DoublyQuotedThings.
+    Export TR LC PP PRP PreL'.
+    Definition qbox_Ui' : Ast.universe := 1.
+    Definition qbox_Ui := Ast.sType qbox_Ui'.
+
+    (*Global Instance has_type_qPreterm {Γ}
+    : has_type Γ ‘Preterm’ (Ast.tSort (Ast.sType 1))
+      := _.
+
+    Definition wttPreterm {Γ} : box' Γ (Ast.tSort (Ast.sType 1))
+      := (‘Preterm’; has_type_qPreterm).
+    Notation "‘‘Preterm’’" := wttPreterm : well_typed_term_scope.*)
+
+    Global Instance has_type_qbox
+    : has_type ε ‘□’ (term' ‘→’ Ast.tSort qbox_Ui).
+    Proof.
+      unfold qbox, qbox_Ui.
+      repeat t_has_type; shelve_unifiable.
+      admit'.
     Qed.
-  End context.
 
-  Definition App : forall {A' B'} {H : is_closed B'},
-                     □ (A' ‘→’ B') -> □ A' -> □ B'.
-  Proof.
-    intros A' B' H AtoB A.
-    refine (AtoB.1 ‘’ A.1;
-            _ (has_type_tApp ε AtoB.1 Ast.nAnon A' B' A.1 AtoB.2 A.2)).
-    clear -H; abstract (hnf in H; rewrite H; intro; assumption).
-  Defined.
-End LA.
+    Axiom box_qtProd_dom_precompose
+    : forall {Γ} A B C,
+        (box' Γ (‘□’ ‘’ B) -> box' Γ (‘□’ ‘’ A))
+        -> box' Γ (‘□’ ‘’ (A ‘‘→’’ C))
+        -> box' Γ (‘□’ ‘’ (B ‘‘→’’ C)).
 
-Module DQT <: DoublyQuotedThings.
-  Export TR LC PP PRP PreL'.
-  Definition qbox_Ui' : Ast.universe := 1.
-  Definition qbox_Ui := Ast.sType qbox_Ui'.
+    (** FIXME: This seems a bit fishy... *)
+    Axiom box_quote_app_quote
+    : forall Γ T,
+        box' Γ (‘□’
+                 ‘’ (‘App’ ‘’ ⌜‘□’ ⌝ ‘’ (‘App’ ‘’ ⌜T ⌝ ‘’ (‘App’ ‘’ ⌜ ‘quote’ ⌝ ‘’ ⌜ T ⌝))))
+        -> box' Γ (‘□’ ‘’ (‘App’ ‘’ ⌜‘□’ ⌝ ‘’ (‘App’ ‘’ ⌜T ⌝ ‘’ ⌜ ⌜ T ⌝ ⌝))).
 
-  Global Instance has_type_qPreterm {Γ}
-  : has_type Γ ‘Preterm’ (Ast.tSort Ast.sSet)
-    := _.
-  Definition wttPreterm {Γ} : box' Γ (Ast.tSort Ast.sSet)
-    := (‘Preterm’; has_type_qPreterm).
-  Notation "‘‘Preterm’’" := wttPreterm : well_typed_term_scope.
+    Axiom box_quote_app_quote_inv
+    : forall Γ T,
+        box' Γ (‘□’ ‘’ (‘App’ ‘’ ⌜‘□’ ⌝ ‘’ (‘App’ ‘’ ⌜T ⌝ ‘’ ⌜ ⌜ T ⌝ ⌝)))
+        -> box' Γ (‘□’
+                    ‘’ (‘App’ ‘’ ⌜‘□’ ⌝ ‘’ (‘App’ ‘’ ⌜T ⌝ ‘’ (‘App’ ‘’ ⌜ ‘quote’ ⌝ ‘’ ⌜ T ⌝)))).
 
-  Global Instance has_type_qbox
-  : has_type ε ‘□’ (term' ‘→’ Ast.tSort qbox_Ui).
-  Proof.
-    unfold qbox, qbox_Ui.
-    repeat t_has_type; shelve_unifiable.
-    admit'.
-  Qed.
+    Quote Definition has_type' := has_type nil.
+    Axiom has_type_has_type' : forall {Γ}, has_type Γ has_type' (‘Preterm’ ‘→’ ‘Preterm’ ‘→’ Ast.tSort (Ast.sType 3)).
+    Existing Instance has_type_has_type'.
+    Definition wtthas_type {Γ} : box' Γ _
+      := (has_type'; has_type_has_type').
+    Notation "‘‘has_type’’" := wtthas_type : well_typed_term_scope.
 
-  Axiom box_qtProd_dom_precompose
-  : forall {Γ} A B C,
-      (box' Γ (‘□’ ‘’ B) -> box' Γ (‘□’ ‘’ A))
-      -> box' Γ (‘□’ ‘’ (A ‘‘→’’ C))
-      -> box' Γ (‘□’ ‘’ (B ‘‘→’’ C)).
+    (*Definition wttexistT {Γ U1 U2} : box' Γ _
+      := (‘existT’; has_type_qexistT _ U1 U2).
+    Notation "‘‘existT’’" := wttexistT : well_typed_term_scope.*)
 
-  (** FIXME: This seems a bit fishy... *)
-  Axiom box_quote_app_quote
-  : forall Γ T,
-      box' Γ (‘□’
-               ‘’ (‘App’ ‘’ ⌜‘□’ ⌝ ‘’ (‘App’ ‘’ ⌜T ⌝ ‘’ (‘App’ ‘’ ⌜ ‘quote’ ⌝ ‘’ ⌜ T ⌝))))
-      -> box' Γ (‘□’ ‘’ (‘App’ ‘’ ⌜‘□’ ⌝ ‘’ (‘App’ ‘’ ⌜T ⌝ ‘’ ⌜ ⌜ T ⌝ ⌝))).
-
-  Axiom box_quote_app_quote_inv
-  : forall Γ T,
-      box' Γ (‘□’ ‘’ (‘App’ ‘’ ⌜‘□’ ⌝ ‘’ (‘App’ ‘’ ⌜T ⌝ ‘’ ⌜ ⌜ T ⌝ ⌝)))
-      -> box' Γ (‘□’
-                  ‘’ (‘App’ ‘’ ⌜‘□’ ⌝ ‘’ (‘App’ ‘’ ⌜T ⌝ ‘’ (‘App’ ‘’ ⌜ ‘quote’ ⌝ ‘’ ⌜ T ⌝)))).
-
-  Quote Definition has_type' := has_type nil.
-  Axiom has_type_has_type' : forall {Γ}, has_type Γ has_type' (‘Preterm’ ‘→’ ‘Preterm’ ‘→’ Ast.tSort (Ast.sType 3)).
-  Existing Instance has_type_has_type'.
-  Definition wtthas_type {Γ} : box' Γ _
-    := (has_type'; has_type_has_type').
-  Notation "‘‘has_type’’" := wtthas_type : well_typed_term_scope.
-
-  Definition wttexistT {Γ U1 U2} : box' Γ _
-    := (‘existT’; has_type_qexistT _ U1 U2).
-  Notation "‘‘existT’’" := wttexistT : well_typed_term_scope.
-
-  Local Ltac set_evars :=
-    repeat match goal with
-             | [ |- appcontext[?E] ] => is_evar E; let e := fresh in set (e := E)
-           end.
-
-  Local Ltac subst_body :=
-    repeat match goal with
-             | [ H := _ |- _ ] => subst H
-           end.
-
-  Local Ltac conv_rewrite
-    := set_evars;
+    Local Ltac set_evars :=
       repeat match goal with
-               | [ |- convertible _ ?x ?x ] => reflexivity
-               | [ |- convertible _ (?x ‘’ _) (?x ‘’ _) ]
-                 => apply tApp_Proper_convertible; [ reflexivity | ]
-               | [ |- convertible _ (_ ‘‘→’’ _) (_ ‘‘→’’ _) ]
-                 => apply qtProd_Proper_convertible
-               | [ |- convertible _ (_ ‘→’ ?x) _ ]
-                 => apply tProd_Proper_convertible; [ | reflexivity ]
-               | _ => progress rewrite_strat repeat (topdown repeat (hints convdb))
-             (*| _ => progress rewrite ?convertible__capture_avoiding_subst_0__tApp, ?convertible__qtApp__closed, ?convertible__quote__closed, ?convertible__quote__app, ?convertible__capture_avoiding_subst_0__tVar0, ?convertible__qquote__closed, ?convertible__capture_avoiding_subst_0__qtProd, ?convertible__quote__qtProd, ?convertible_beta_app_lambda*)
-             end;
-      subst_body.
-
-  Local Notation "x ‘’ y" := (wttApp_1 x%wtt y%wtt) : well_typed_term_scope.
-
-  Definition Quot : forall T, □ T -> □ (‘□’ ‘’ ⌜ T ⌝).
-  Proof.
-    intros T bT.
-    unfold qbox.
-    eapply box'_respectful; cycle 1.
-    2:unfold tApp.
-    2:let RHS := match goal with |- ?R ?x ?y => constr:y end in
-      match RHS with
-        | context G[Ast.tApp (Ast.tLambda ?x ?A ?b) [?a]]
-          => let G' := context G[subst_n_name b a (Some 0%nat) x] in
-             refine (@transitivity _ _ _ _ G' _ _ _); simpl
-      end;
-        repeat match goal with
-                 | [ |- ?R (Ast.tApp _ _) (Ast.tApp _ _) ]
-                   => apply tApp_Proper
-                 | [ |- ?R _ (Ast.tApp (Ast.tLambda _ _ _) _) ]
-                   => etransitivity; [ | symmetry; apply conv_beta ]
-                 | [ |- ?R (Ast.tLambda ?n ?A _) (Ast.tLambda ?n ?A _) ]
-                   => apply tLambda_Proper1
-                 | [ |- ?R ?x ?x ] => reflexivity
-                 | [ |- (_ * _)%type ] => split
-                 | [ |- True ] => constructor
-                 | _ => progress simpl
-               end.
-    Timeout 5 refine (‘‘existT’’ ‘’ ‘‘Preterm’’ ‘’ (wttLambda_nd _ (‘‘has_type’’ ‘’ ‘‘VAR₀’’ ‘’ ‘⌜ T ⌝’)) ‘’ ‘⌜ bT.1 ⌝’ ‘’ (_ bT.2))%wtt; shelve_unifiable.
-    2:repeat match goal with
-               | [ |- ?R (Ast.tApp _ [_]) (Ast.tApp _ [_]) ]
-                 => apply tApp_Proper
-               | [ |- ?R (Ast.tApp _ nil) (Ast.tApp _ nil) ]
-                 => apply tApp_Proper
-               | [ |- ?R (Ast.tApp _ [_;_]) (Ast.tApp _ [_;_]) ]
-                 => apply tApp_Proper
-               | [ |- ?R (Ast.tApp _ [_;_;_]) (Ast.tApp _ [_;_;_]) ]
-                 => apply tApp_Proper
-               | [ |- ?R _ (Ast.tApp (Ast.tLambda _ _ _) _) ]
-                 => etransitivity; [ | symmetry; apply conv_beta ]
-               | [ |- ?R (Ast.tApp (Ast.tApp _ _) _) _ ]
-                 => apply conv_tApp_cons2
-               | [ |- ?R _ (Ast.tApp (Ast.tApp _ _) _) ]
-                 => symmetry; apply conv_tApp_cons2; symmetry
-               | [ |- ?R (Ast.tLambda ?n ?A _) (Ast.tLambda ?n ?A _) ]
-                 => apply tLambda_Proper1
-               | [ |- ?R _ (Ast.tLambda (Ast.nNamed _) _ _) ]
-                 => etransitivity; [ | symmetry; apply conv_tLambda_unname ]
-               | [ |- ?R ?x ?x ] => reflexivity
-               | [ |- (_ * _)%type ] => split
-               | [ |- True ] => constructor
-               | _ => progress simpl
-               | _ => progress unfold quote_term.quote, term_quotable
-               | _ => rewrite eq__quote_term__closed_helper
+               | [ |- appcontext[?E] ] => is_evar E; let e := fresh in set (e := E)
              end.
-    { simpl.
-      intro ht.
-      eapply box'_respectful.
-      { let RHS := match goal with |- ?R ?x ?y => constr:y end in
+
+    Local Ltac subst_body :=
+      repeat match goal with
+               | [ H := _ |- _ ] => subst H
+             end.
+
+    Local Ltac conv_rewrite
+      := set_evars;
+        repeat match goal with
+                 | [ |- convertible _ ?x ?x ] => reflexivity
+                 | [ |- convertible _ (?x ‘’ _) (?x ‘’ _) ]
+                   => apply tApp_Proper_convertible; [ reflexivity | ]
+                 | [ |- convertible _ (_ ‘‘→’’ _) (_ ‘‘→’’ _) ]
+                   => apply qtProd_Proper_convertible
+                 | [ |- convertible _ (_ ‘→’ ?x) _ ]
+                   => apply tProd_Proper_convertible; [ | reflexivity ]
+                 | _ => progress rewrite_strat repeat (topdown repeat (hints convdb))
+               (*| _ => progress rewrite ?convertible__capture_avoiding_subst_0__tApp, ?convertible__qtApp__closed, ?convertible__quote__closed, ?convertible__quote__app, ?convertible__capture_avoiding_subst_0__tVar0, ?convertible__qquote__closed, ?convertible__capture_avoiding_subst_0__qtProd, ?convertible__quote__qtProd, ?convertible_beta_app_lambda*)
+               end;
+        subst_body.
+
+    Local Notation "x ‘’ y" := (wttApp_1 x%wtt y%wtt) : well_typed_term_scope.
+
+    Definition Quot : forall T, □ T -> □ (‘□’ ‘’ ⌜ T ⌝).
+    Proof.
+      intros T bT.
+      unfold qbox.
+      eapply box'_respectful; cycle 1.
+      2:unfold tApp.
+      2:let RHS := match goal with |- ?R ?x ?y => constr:y end in
         match RHS with
           | context G[Ast.tApp (Ast.tLambda ?x ?A ?b) [?a]]
             => let G' := context G[subst_n_name b a (Some 0%nat) x] in
                refine (@transitivity _ _ _ _ G' _ _ _); simpl
         end;
           repeat match goal with
+                   | [ |- ?R (Ast.tApp _ _) (Ast.tApp _ _) ]
+                     => apply tApp_Proper
                    | [ |- ?R _ (Ast.tApp (Ast.tLambda _ _ _) _) ]
                      => etransitivity; [ | symmetry; apply conv_beta ]
-                   | [ |- ?R (Ast.tApp (Ast.tLambda _ _ _) _) _ ]
-                     => etransitivity; [ apply conv_beta | ]
                    | [ |- ?R (Ast.tLambda ?n ?A _) (Ast.tLambda ?n ?A _) ]
                      => apply tLambda_Proper1
-                   | [ |- ?R (Ast.tApp _ [_]) (Ast.tApp _ [_]) ]
-                     => apply tApp_Proper
-                   | [ |- ?R (Ast.tApp _ nil) (Ast.tApp _ nil) ]
-                     => apply tApp_Proper
-                   | [ |- ?R (Ast.tApp _ [_;_]) (Ast.tApp _ [_;_]) ]
-                     => apply tApp_Proper
-                   | [ |- ?R (Ast.tApp _ [_;_;_]) (Ast.tApp _ [_;_;_]) ]
-                     => apply tApp_Proper
-                   | [ |- ?R (Ast.tApp (Ast.tApp _ _) _) _ ]
-                     => apply conv_tApp_cons2
-                   | [ |- ?R _ (Ast.tApp (Ast.tApp _ _) _) ]
-                     => symmetry; apply conv_tApp_cons2; symmetry
                    | [ |- ?R ?x ?x ] => reflexivity
                    | [ |- (_ * _)%type ] => split
                    | [ |- True ] => constructor
                    | _ => progress simpl
-                   | _ => progress unfold quote_term.quote, term_quotable
-                   | _ => rewrite eq__quote_term__closed_helper
-                 end;
-          reflexivity. }
-      admit.
-  Admitted.
+                 end.
+      Timeout 5 refine (‘‘existT’’ ‘’ ‘‘Preterm’’ ‘’ (wttLambda_nd _ (‘‘has_type’’ ‘’ ‘‘VAR₀’’ ‘’ ‘⌜ T ⌝’)) ‘’ ‘⌜ bT.1 ⌝’ ‘’ (_ bT.2))%wtt; shelve_unifiable.
+      2:repeat match goal with
+                 | [ |- ?R (Ast.tApp _ [_]) (Ast.tApp _ [_]) ]
+                   => apply tApp_Proper
+                 | [ |- ?R (Ast.tApp _ nil) (Ast.tApp _ nil) ]
+                   => apply tApp_Proper
+                 | [ |- ?R (Ast.tApp _ [_;_]) (Ast.tApp _ [_;_]) ]
+                   => apply tApp_Proper
+                 | [ |- ?R (Ast.tApp _ [_;_;_]) (Ast.tApp _ [_;_;_]) ]
+                   => apply tApp_Proper
+                 | [ |- ?R _ (Ast.tApp (Ast.tLambda _ _ _) _) ]
+                   => etransitivity; [ | symmetry; apply conv_beta ]
+                 | [ |- ?R (Ast.tApp (Ast.tApp _ _) _) _ ]
+                   => apply conv_tApp_cons2
+                 | [ |- ?R _ (Ast.tApp (Ast.tApp _ _) _) ]
+                   => symmetry; apply conv_tApp_cons2; symmetry
+                 | [ |- ?R (Ast.tLambda ?n ?A _) (Ast.tLambda ?n ?A _) ]
+                   => apply tLambda_Proper1
+                 | [ |- ?R _ (Ast.tLambda (Ast.nNamed _) _ _) ]
+                   => etransitivity; [ | symmetry; apply conv_tLambda_unname ]
+                 | [ |- ?R ?x ?x ] => reflexivity
+                 | [ |- (_ * _)%type ] => split
+                 | [ |- True ] => constructor
+                 | _ => progress simpl
+                 | _ => progress unfold quote_term.quote, term_quotable
+                 | _ => rewrite eq__quote_term__closed_helper
+               end.
+      { simpl.
+        intro ht.
+        eapply box'_respectful.
+        { let RHS := match goal with |- ?R ?x ?y => constr:y end in
+          match RHS with
+            | context G[Ast.tApp (Ast.tLambda ?x ?A ?b) [?a]]
+              => let G' := context G[subst_n_name b a (Some 0%nat) x] in
+                 refine (@transitivity _ _ _ _ G' _ _ _); simpl
+          end;
+            repeat match goal with
+                     | [ |- ?R _ (Ast.tApp (Ast.tLambda _ _ _) _) ]
+                       => etransitivity; [ | symmetry; apply conv_beta ]
+                     | [ |- ?R (Ast.tApp (Ast.tLambda _ _ _) _) _ ]
+                       => etransitivity; [ apply conv_beta | ]
+                     | [ |- ?R (Ast.tLambda ?n ?A _) (Ast.tLambda ?n ?A _) ]
+                       => apply tLambda_Proper1
+                     | [ |- ?R (Ast.tApp _ [_]) (Ast.tApp _ [_]) ]
+                       => apply tApp_Proper
+                     | [ |- ?R (Ast.tApp _ nil) (Ast.tApp _ nil) ]
+                       => apply tApp_Proper
+                     | [ |- ?R (Ast.tApp _ [_;_]) (Ast.tApp _ [_;_]) ]
+                       => apply tApp_Proper
+                     | [ |- ?R (Ast.tApp _ [_;_;_]) (Ast.tApp _ [_;_;_]) ]
+                       => apply tApp_Proper
+                     | [ |- ?R (Ast.tApp (Ast.tApp _ _) _) _ ]
+                       => apply conv_tApp_cons2
+                     | [ |- ?R _ (Ast.tApp (Ast.tApp _ _) _) ]
+                       => symmetry; apply conv_tApp_cons2; symmetry
+                     | [ |- ?R ?x ?x ] => reflexivity
+                     | [ |- (_ * _)%type ] => split
+                     | [ |- True ] => constructor
+                     | _ => progress simpl
+                     | _ => progress unfold quote_term.quote, term_quotable
+                     | _ => rewrite eq__quote_term__closed_helper
+                   end;
+            reflexivity. }
+        admit.
+    Admitted.
 
 
-  Section context.
-    Context (qX qL0 : Preterm).
-    Let Γ := (ε ▻ (‘□’
-                    ‘’ (tLambda ‘Preterm’
-                                (‘App’ ‘’ ⌜ ‘□’ ⌝
-                                  ‘’ (‘App’ ‘’ ‘VAR₀’ ‘’ (‘App’ ‘’ ⌜ ‘quote’ ⌝ ‘’ ‘VAR₀’))
-                                  ‘‘→’’ ⌜ qX ⌝) ‘’ ⌜ qL0 ⌝))).
+    Section context.
+      Context (qX qL0 : Preterm).
+      Let Γ := (ε ▻ (‘□’
+                      ‘’ (tLambda ‘Preterm’
+                                  (‘App’ ‘’ ⌜ ‘□’ ⌝
+                                    ‘’ (‘App’ ‘’ ‘VAR₀’ ‘’ (‘App’ ‘’ ⌜ ‘quote’ ⌝ ‘’ ‘VAR₀’))
+                                    ‘‘→’’ ⌜ qX ⌝) ‘’ ⌜ qL0 ⌝))).
 
-    Axiom qQuote
-    : forall T,
-        let A := (‘□’ ‘’ T)%preterm in
-        box' Γ (A ‘→’ (‘□’ ‘’ (⌜ A ⌝))).
+      Axiom qQuote
+      : forall T,
+          let A := (‘□’ ‘’ T)%preterm in
+          box' Γ (A ‘→’ (‘□’ ‘’ (⌜ A ⌝))).
 
-    Axiom qbApp
-    : forall A' B',
-        box' Γ ((‘□’ ‘’ (A' ‘‘→’’ B')) ‘→’ (‘□’ ‘’ A') ‘→’ (‘□’ ‘’ B')).
-  End context.
-End DQT.
+      Axiom qbApp
+      : forall A' B',
+          box' Γ ((‘□’ ‘’ (A' ‘‘→’’ B')) ‘→’ (‘□’ ‘’ A') ‘→’ (‘□’ ‘’ B')).
+    End context.
+  End DQT.
 
-Declare Module LH : LobHypotheses LC.
+  Declare Module LH : LobHypotheses LC.
 
-Module Lob <: LobsTheorem LC LH.
-  Module PRTR' := PRTR DQT.
-  Module LA' := LA DQT.
-  Module Lob' := LobOfPreLob LC LH PP PreL' PRP TR PRTR' LA'.
-  Definition lob := Lob'.lob.
-  Print Assumptions lob.
-End Lob.
+  Module Lob <: LobsTheorem LC LH.
+    Module PRTR' := PRTR DQT.
+    Module LA' := LA DQT.
+    Module Lob' := LobOfPreLob LC LH PP PreL' PRP TR PRTR' LA'.
+    Definition lob := Lob'.lob.
+    Print Assumptions lob.
+  End Lob.
 
-Print Assumptions Lob.lob.
+  Print Assumptions Lob.lob.
