internal/conversion_quote.v
@@ -1,0 +1,367 @@
+Require Import Coq.Setoids.Setoid Coq.Classes.CMorphisms.
+Require Export Lob.Notations.
+
+Require Import Template.Template.
+
+Require Import Coq.Strings.String.
+Require Import Coq.Program.Program.
+Require Import Coq.PArith.BinPos.
+Local Open Scope string_scope.
+Local Open Scope positive_scope.
+
+Require Export Lob.quote_term.
+(*Require Export Lob.quote_has_type.*)
+Require Export Lob.conversion.
+
+Notation "( x ; y )" := (existT _ x y).
+Notation "x .1" := (projT1 x) (at level 3, format "x '.1'").
+Notation "x .2" := (projT2 x) (at level 3, format "x '.2'").
+
+Tactic Notation "unique" "pose" "proof" constr(defn) :=
+  let T := type of defn in
+  match goal with
+    | [ H : T |- _ ] => fail 1
+    | _ => pose proof defn
+  end.
+
+(** Test if a tactic succeeds, but always roll-back the results *)
+Tactic Notation "test" tactic3(tac) :=
+  try (first [ tac | fail 2 tac "does not succeed" ]; fail 0 tac "succeeds"; [](* test for [t] solved all goals *)).
+
+(** [not tac] is equivalent to [fail tac "succeeds"] if [tac] succeeds, and is equivalent to [idtac] if [tac] fails *)
+Tactic Notation "not" tactic3(tac) := try ((test tac); fail 1 tac "succeeds").
+
+
+Section quote_subst_eq.
+  Create HintDb t_quote_db discriminated.
+
+  Local Ltac t_quote0 tac :=
+    repeat match goal with
+             | _ => progress simpl
+             | _ => progress intros
+             | _ => reflexivity
+             | [ |- Ast.tApp _ _ = Ast.tApp _ _ ] => apply f_equal2; [ solve [ tac ] | ]
+             | [ |- Ast.tApp _ _ = Ast.tApp _ _ ] => apply f_equal2; [ | solve [ tac ] ]
+             | [ |- cons _ _ = cons _ _ ] => apply f_equal2
+             (*| _ => apply tApp_Proper_convertible; [ solve [ tac ] | ]
+             | _ => apply tApp_Proper_convertible; [ | solve [ tac ] ]
+             | [ |- convertible _ (Ast.tApp _ (_::_::_)%list) _ ] => apply conv_tApp_cons1
+             | [ |- convertible _ _ (Ast.tApp _ (_::_::_)%list) ] => symmetry; apply conv_tApp_cons1; symmetry*)
+             | _ => progress change conversion.convertible with convertible
+           end.
+  Local Ltac t_quote :=
+    repeat match goal with
+             | _ => progress t_quote0 t_quote
+             | _ => solve [ eauto with nocore t_quote_db ]
+           end.
+
+  Definition eq__quote_nat__closed_helper {A x}
+  : forall n n', eq (subst_n_name (quote_nat A) x n n') (quote_nat A).
+  Proof. induction A; t_quote. Qed.
+
+  Hint Resolve eq__quote_nat__closed_helper : t_quote_db.
+
+  Definition eq__quote_bool__closed_helper {A x}
+  : forall n n', eq (subst_n_name (quote_bool A) x n n') (quote_bool A).
+  Proof. induction A; t_quote. Qed.
+
+  Hint Resolve eq__quote_bool__closed_helper : t_quote_db.
+
+  Definition eq__quote_ascii__closed_helper {A x}
+  : forall n n', eq (subst_n_name (quote_ascii A) x n n') (quote_ascii A).
+  Proof. induction A; t_quote. Qed.
+
+  Hint Resolve eq__quote_ascii__closed_helper : t_quote_db.
+
+  Definition eq__quote_ident__closed_helper {A x}
+  : forall n n', eq (subst_n_name (quote_ident A) x n n') (quote_ident A).
+  Proof. induction A; t_quote. Qed.
+
+  Hint Resolve eq__quote_ident__closed_helper : t_quote_db.
+
+  Definition eq__quote_positive__closed_helper {A x}
+  : forall n n', eq (subst_n_name (quote_positive A) x n n') (quote_positive A).
+  Proof. induction A; t_quote. Qed.
+
+  Hint Resolve eq__quote_positive__closed_helper : t_quote_db.
+
+  Definition eq__quote_sort__closed_helper {A x}
+  : forall n n', eq (subst_n_name (quote_sort A) x n n') (quote_sort A).
+  Proof. induction A; t_quote. Qed.
+
+  Hint Resolve eq__quote_sort__closed_helper : t_quote_db.
+
+  Definition eq__quote_cast_kind__closed_helper {A x}
+  : forall n n', eq (subst_n_name (quote_cast_kind A) x n n') (quote_cast_kind A).
+  Proof. induction A; t_quote. Qed.
+
+  Hint Resolve eq__quote_cast_kind__closed_helper : t_quote_db.
+
+  Definition eq__quote_name__closed_helper {A x}
+  : forall n n', eq (subst_n_name (quote_name A) x n n') (quote_name A).
+  Proof. induction A; t_quote. Qed.
+
+  Hint Resolve eq__quote_name__closed_helper : t_quote_db.
+
+  Definition eq__quote_inductive__closed_helper {A x}
+  : forall n n', eq (subst_n_name (quote_inductive A) x n n') (quote_inductive A).
+  Proof. induction A; t_quote. Qed.
+
+  Hint Resolve eq__quote_inductive__closed_helper : t_quote_db.
+
+  Section sub_helpers.
+    Context (eq__quote_term__closed_helper : forall (A x : Ast.term)
+                                                    (n : option nat)
+                                                    (n' : Ast.name),
+                                               eq
+                                                 (subst_n_name
+                                                    (quote_term A) x n n')
+                                                 (quote_term A)).
+
+    Fixpoint eq__quote_term_helper__closed_helper ls x
+    : forall n n', eq (subst_n_name (quote_term_helper quote_term ls) x n n') (quote_term_helper quote_term ls).
+    Proof.
+      destruct ls as [|y ys]; simpl; try reflexivity; [].
+      intros n n'.
+      t_quote.
+    Defined.
+
+    Fixpoint eq__quote_term_helper_def__closed_helper ls x
+    : forall n n', eq (subst_n_name (quote_term_helper_def quote_term ls) x n n') (quote_term_helper_def quote_term ls).
+    Proof.
+      destruct ls as [|[] ys]; simpl; try reflexivity; [].
+      intros n n'.
+      t_quote.
+    Defined.
+  End sub_helpers.
+
+  Fixpoint eq__quote_term__closed_helper A x {struct A}
+  : forall n n', eq (subst_n_name (quote_term A) x n n') (quote_term A).
+  Proof.
+    intros n n'; destruct A; simpl;
+    repeat match goal with
+             | [ ls : list Ast.term |- _ ]
+               => unique pose proof (eq__quote_term_helper__closed_helper eq__quote_term__closed_helper ls x n n')
+             | [ ls : Ast.mfixpoint Ast.term |- _ ]
+               => unique pose proof (eq__quote_term_helper_def__closed_helper eq__quote_term__closed_helper ls x n n')
+             | [ A : Ast.term |- _ ]
+               => not constr_eq A x; unique pose proof (eq__quote_term__closed_helper A x n n')
+           end;
+    try solve [ t_quote ].
+  Defined.
+End quote_subst_eq.
+
+Section quote_has_type.
+  Local Ltac t_quote0 tac :=
+    repeat match goal with
+             | _ => progress simpl
+             | _ => progress intros
+             | _ => reflexivity
+             | [ |- has_type ?Γ (Ast.tApp ?f [?a]) ?B ]
+               => eapply (fun A => @has_type_tApp Γ f Ast.nAnon A B a)
+             | [ |- has_type ?Γ (Ast.tApp ?f [?a]) ?B ]
+               => refine (@has_type_tApp Γ f Ast.nAnon _ _ a _ _); shelve_unifiable
+             | [ |- has_type ?Γ (Ast.tApp _ (_::_::_)%list) _ ]
+               => apply has_type_tApp_split
+             | [ |- has_type (_ ▻▻ _) _ _ ]
+               => apply wkg_rel_free; [ intros ? [?|]; reflexivity | intros ? [?|]; reflexivity | ]
+             | [ |- has_type _ _ _ ]
+               => eapply has_type_conv_subst;
+                 [ eapply has_type_tConstruct1_Lookup;
+                   [ | | simpl; reflexivity ];
+                   hnf; simpl; reflexivity
+                 | ]
+             | [ |- convertible ?Γ ?k _ ] => unfold k
+             | [ |- convertible ?Γ (Ast.tConst ?n) _ ]
+               => let H := fresh in
+                  pose proof (@conv_delta_Lookup Γ n) as H;
+                    unfold is_rel_free in H;
+                    simpl in H;
+                    apply (H (fun _ _ => eq_refl))
+             | [ |- conversion.convertible _ (Ast.tProd _ _ _) (Ast.tProd _ _ _) ]
+               => apply conv_tProd_respectful
+             | _ => exact _
+           end.
+  Local Ltac t_quote :=
+    repeat match goal with
+             | _ => progress t_quote0 t_quote
+             | _ => solve [ eauto with nocore ]
+           end.
+
+  Global Instance has_type__quote__nil A T (H : forall Γ, has_type (DefaultContext ▻▻ Γ) A T)
+  : has_type DefaultContext A T
+    := H nil.
+
+  Global Instance has_type__quote_nat A
+  : forall Γ, has_type (DefaultContext ▻▻ Γ) (quote_nat A) nat'.
+  Proof. induction A; t_quote. Qed.
+
+  Global Instance has_type__quote_bool A
+  : forall Γ, has_type (DefaultContext ▻▻ Γ) (quote_bool A) bool'.
+  Proof. induction A; t_quote. Qed.
+
+  Global Instance has_type__quote_ascii A
+  : forall Γ, has_type (DefaultContext ▻▻ Γ) (quote_ascii A) ascii'.
+  Proof. induction A; t_quote. Qed.
+
+  Global Instance has_type__quote_ident A
+  : forall Γ, has_type (DefaultContext ▻▻ Γ) (quote_ident A) ident'.
+  Proof. induction A; t_quote. Qed.
+
+  Global Instance has_type__quote_positive A
+  : forall Γ, has_type (DefaultContext ▻▻ Γ) (quote_positive A) positive'.
+  Proof. induction A; t_quote. Qed.
+
+  Global Instance has_type__quote_sort A
+  : forall Γ, has_type (DefaultContext ▻▻ Γ) (quote_sort A) sort'.
+  Proof. induction A; t_quote. Qed.
+
+  Global Instance has_type__quote_cast_kind A
+  : forall Γ, has_type (DefaultContext ▻▻ Γ) (quote_cast_kind A) cast_kind'.
+  Proof. induction A; t_quote. Qed.
+
+  Global Instance has_type__quote_name A
+  : forall Γ, has_type (DefaultContext ▻▻ Γ) (quote_name A) name'.
+  Proof. induction A; t_quote. Qed.
+
+  Global Instance has_type__quote_inductive A
+  : forall Γ, has_type (DefaultContext ▻▻ Γ) (quote_inductive A) inductive'.
+  Proof. induction A; t_quote. Qed.
+
+  Local Ltac t_has_type' :=
+    idtac;
+    match goal with
+      | [ |- has_type ?Γ (Ast.tApp ?f [?a]) ?B ]
+        => refine (@has_type_tApp Γ f Ast.nAnon _ _ a _ _); shelve_unifiable
+      | _ => progress simpl
+      | _ => exact _
+      | _ => apply has_type_tApp_split
+      | [ |- has_type _ (quote_term _) (subst_n_name ?e _ _ _) ]
+        => progress unify e term'
+      | [ |- convertible ?Γ (Ast.tApp (Ast.tConst ?n) _) _ ]
+        => let H := fresh in
+           pose proof (@conv_delta_Lookup Γ n) as H;
+             unfold is_rel_free in H;
+             simpl in H;
+             etransitivity; [ apply conv_tApp_respectful; [ apply H; intros ? [?|]; simpl; reflexivity | reflexivity ] | ];
+             clear H
+      | [ |- has_type ?Γ (Ast.tApp ?f [?a]) ?B ]
+        => let A := fresh in
+           let B' := fresh in
+           evar (A : Ast.term);
+             evar (B' : Ast.term);
+             let H := fresh in
+             pose proof (@has_type_tApp Γ f Ast.nAnon A B' a) as H;
+               subst A B';
+               refine (_ (H _ _)); shelve_unifiable; clear H;
+               [ | repeat t_has_type' | ]; shelve_unifiable;
+               [ simpl; solve [ exact (fun x => x)
+                              | let H' := fresh in
+                                intro H';
+                                  eapply has_type_conv_subst; [ | solve [ apply conv_tProd_unname ] ];
+                                  exact H' ]
+               | .. ]
+      | [ |- has_type (_ ▻▻ _) _ _ ]
+        => apply wkg_rel_free; [ intros ? [?|]; reflexivity | intros ? [?|]; reflexivity | ]
+      | [ |- has_type _ _ _ ]
+        => eapply has_type_conv_subst;
+          [ eapply has_type_tConstruct1_Lookup;
+            [ | | simpl; reflexivity ];
+            hnf; simpl;
+            [ reflexivity | intros ? [?|]; simpl; reflexivity ]
+          | ]
+      | [ |- has_type _ _ _ ]
+        => eapply has_type_conv_subst;
+          [ eapply has_type_tInd1_Lookup;
+            [ | | simpl; reflexivity ];
+            hnf; simpl;
+            [ reflexivity | intros ? [?|]; simpl; reflexivity ]
+          | ]
+      | [ |- convertible ?Γ ?k _ ] => unfold k
+      | [ |- convertible ?Γ (Ast.tConst ?n) _ ]
+        => let H := fresh in
+           pose proof (@conv_delta_Lookup Γ n) as H;
+             unfold is_rel_free in H;
+             simpl in H;
+             apply (H (fun _ _ => eq_refl))
+      | [ |- conversion.convertible _ (Ast.tProd _ _ _) (Ast.tProd _ _ _) ]
+        => apply conv_tProd_respectful
+      | [ |- convertible _ (Ast.tProd (Ast.nNamed _) _ _) _ ]
+        => etransitivity; [ solve [ apply conv_tProd_unname ] | ]
+      | [ |- convertible _ _ ?e ]
+        => is_evar e; reflexivity
+      | [ |- convertible _ ?e ?e ]
+        => reflexivity
+      | [ |- context[Ast.tApp (Ast.tLambda _ _ _) [_]] ]
+        => etransitivity; [ solve [ eapply conv_beta ] | ]; simpl
+    end.
+  Local Ltac t_has_type := repeat t_has_type'.
+
+  Local Notation Γ := (List.map (fun nT => CBinder (fst nT) (snd nT))) (only parsing).
+  Section sub_helpers.
+    Context (has_type__quote_term : forall (A : Ast.term),
+                                      forall nTs, has_type (DefaultContext ▻▻ Γ nTs) (quote_term A) term').
+
+    Fixpoint has_type__quote_term_helper ls
+    : forall nTs, has_type (DefaultContext ▻▻ Γ nTs) (quote_term_helper quote_term ls) (Ast.tApp list' [term']).
+    Proof.
+      destruct ls as [|y ys]; simpl.
+      { intros; t_has_type. }
+      { intros nTs.
+        specialize (fun nTs => has_type__quote_term_helper ys nTs).
+        specialize (fun nTs => has_type__quote_term y nTs).
+        induction nTs.
+        { specialize (has_type__quote_term_helper nil).
+          specialize (has_type__quote_term nil).
+          simpl in *.
+          t_has_type. }
+        { simpl.
+          apply (@wkg_rel_free _ [_]%list);
+            [ intros ? [?|]; simpl;
+              rewrite ?eq__quote_term_helper__closed_helper, ?eq__quote_term__closed_helper by apply eq__quote_term__closed_helper;
+              try reflexivity
+            | intros ? [?|]; reflexivity | ].
+          auto with nocore. } }
+    Defined.
+
+    Fixpoint has_type__quote_term_helper_def ls
+    : forall nTs, has_type (DefaultContext ▻▻ Γ nTs) (quote_term_helper_def quote_term ls) (Ast.tApp list' [Ast.tApp def' [term']]).
+    Proof.
+      destruct ls as [|[dnam dtyp dbod] ys]; simpl.
+      { intros; t_has_type. }
+      { intros nTs.
+        specialize (fun nTs => has_type__quote_term_helper_def ys nTs).
+        pose proof (fun nTs => has_type__quote_term dtyp nTs) as has_type__quote_term__dtyp.
+        pose proof (fun nTs => has_type__quote_term dbod nTs) as has_type__quote_term__dbod.
+        clear has_type__quote_term.
+        induction nTs.
+        { specialize (has_type__quote_term_helper_def nil).
+          specialize (has_type__quote_term__dtyp nil).
+          specialize (has_type__quote_term__dbod nil).
+          simpl in *.
+          t_has_type. }
+        { simpl.
+          apply (@wkg_rel_free _ [_]%list);
+            [ intros ? [?|]; simpl;
+              rewrite ?eq__quote_term_helper_def__closed_helper, ?eq__quote_term__closed_helper, ?eq__quote_nat__closed_helper, ?eq__quote_name__closed_helper by apply eq__quote_term__closed_helper;
+              try reflexivity
+            | intros ? [?|]; reflexivity | ].
+          auto with nocore. } }
+    Defined.
+  End sub_helpers.
+
+  Fixpoint has_type__quote_term A {struct A}
+  : forall nTs, has_type (DefaultContext ▻▻ Γ nTs) (quote_term A) term'.
+  Proof.
+    destruct A; t_quote;
+    try solve [ apply has_type__quote_term_helper; assumption
+              | apply has_type__quote_term_helper_def; assumption ];
+    t_quote.
+    t_has_type.
+    t_quote.
+  Qed.
+End quote_has_type.
+
+Global Instance has_type__quote_term_1 A T
+: has_type (DefaultContext ▻ CBinder Ast.nAnon T) (quote_term A) term'
+  := @has_type__quote_term A [(Ast.nAnon, T)].
