internal/Notations.v
@@ -6,3 +6,6 @@ Reserved Notation "Γ ▻ x" (at level 55, right associativity).
 Reserved Notation "Γ ▻▻ Γ'" (at level 60, right associativity).
 Reserved Notation "□ T" (at level 0).
 Reserved Notation "x [ 0 ↦ y ]" (at level 0, no associativity).
+Notation "( x ; y )" := (existT _ x y).
+Notation "x .1" := (projT1 x) (at level 3, format "x '.1'").
+Notation "x .2" := (projT2 x) (at level 3, format "x '.2'").
